@prefix : <http://www.w3id.org/hsu-aut/DINEN61360#> .
@prefix owl: <http://www.w3.org/2002/07/owl#> .
@prefix rdf: <http://www.w3.org/1999/02/22-rdf-syntax-ns#> .
@prefix xml: <http://www.w3.org/XML/1998/namespace> .
@prefix xsd: <http://www.w3.org/2001/XMLSchema#> .
@prefix rdfs: <http://www.w3.org/2000/01/rdf-schema#> .
@base <http://www.w3id.org/hsu-aut/DINEN61360#> .

<http://www.w3id.org/hsu-aut/DINEN61360> rdf:type owl:Ontology ;
                                          owl:versionIRI <http://www.w3id.org/hsu-aut/DINEN61360/2.0.2> ;
                                          rdfs:comment "An ontology based on IEC 61360 standard for structured property modeling. Defines properties with type descriptions and instances having expression goals (requirement, actual_value, assurance, variable) and relational operators for value specification and constraint definition." ;
                                          owl:versionInfo "2.0.2" .

#################################################################
#    Object Properties
#################################################################

###  http://www.w3id.org/hsu-aut/DINEN61360#Data_Element_describes
:Data_Element_describes rdf:type owl:ObjectProperty ;
                        owl:inverseOf :has_Data_Element ;
                        rdfs:domain :Data_Element ;
                        rdfs:comment """Description:
This ObjectProperty is used to connect a data element with any kind of entity that is described by the data element""" .


###  http://www.w3id.org/hsu-aut/DINEN61360#Instance_Description_has_Type
:Instance_Description_has_Type rdf:type owl:ObjectProperty ;
                               owl:inverseOf :Type_Description_has_Instance ;
                               rdfs:domain :Instance_Description ;
                               rdfs:range :Type_Description .


###  http://www.w3id.org/hsu-aut/DINEN61360#Type_Description_has_Instance
:Type_Description_has_Instance rdf:type owl:ObjectProperty ;
                               rdfs:domain :Type_Description ;
                               rdfs:range :Instance_Description .


###  http://www.w3id.org/hsu-aut/DINEN61360#complex_Data_Type_has_Member
:complex_Data_Type_has_Member rdf:type owl:ObjectProperty ;
                              owl:inverseOf :is_Member_of_Complex_Data_Type ;
                              rdfs:domain [ owl:intersectionOf ( :Instance_Description
                                                                 [ rdf:type owl:Restriction ;
                                                                   owl:onProperty :Instance_Description_has_Type ;
                                                                   owl:allValuesFrom :Complex_Data_Type
                                                                 ]
                                                               ) ;
                                            rdf:type owl:Class
                                          ] ;
                              rdfs:range :Complex_Data_Type_Member ;
                              rdfs:comment """Description:
ObjectProperty that is used to connect an instance of a complex data type with corresponding members of the complex data type. These members are connected to types and instances of other (complex) data types""" .


###  http://www.w3id.org/hsu-aut/DINEN61360#has_Data_Element
:has_Data_Element rdf:type owl:ObjectProperty ;
                  rdfs:range :Data_Element ;
                  rdfs:comment """Description:
This ObjectProperty is used to connect any kind of entity with a data element that is used for its description.""" .


###  http://www.w3id.org/hsu-aut/DINEN61360#has_Instance_Description
:has_Instance_Description rdf:type owl:ObjectProperty ;
                          owl:inverseOf :is_Instance_Description_of_Data_Element ;
                          rdf:type owl:InverseFunctionalProperty ;
                          rdfs:domain [ rdf:type owl:Class ;
                                        owl:unionOf ( :Complex_Data_Type_Member
                                                      :Data_Element
                                                    )
                                      ] ;
                          rdfs:range :Instance_Description ;
                          rdfs:comment """Description:
ObjectProperty is used to connect an individual that needs to be described by DataProperties with the Instance Description of that properties.""" .


###  http://www.w3id.org/hsu-aut/DINEN61360#has_Type_Description
:has_Type_Description rdf:type owl:ObjectProperty ;
                      owl:inverseOf :is_Type_Description_of_Data_Element ;
                      rdf:type owl:FunctionalProperty ;
                      rdfs:domain [ rdf:type owl:Class ;
                                    owl:unionOf ( :Complex_Data_Type_Member
                                                  :Data_Element
                                                )
                                  ] ;
                      rdfs:range :Type_Description ;
                      rdfs:comment """Description:
ObjectProperty is used to connect an individual that needs to be described by DataProperties with the Type Description of that properties.

Functional:
Any indivudual representing a property, can have only one Type Description""" .


###  http://www.w3id.org/hsu-aut/DINEN61360#is_Instance_Description_of_Data_Element
:is_Instance_Description_of_Data_Element rdf:type owl:ObjectProperty ;
                                         rdfs:comment """Description:
ObjectProperty is used to connect an Instance Description with the Data_Element that it describes.

Inverse of has_Instance_Description""" .


###  http://www.w3id.org/hsu-aut/DINEN61360#is_Member_of_Complex_Data_Type
:is_Member_of_Complex_Data_Type rdf:type owl:ObjectProperty ;
                                rdfs:domain :Complex_Data_Type_Member ;
                                rdfs:range [ owl:intersectionOf ( :Instance_Description
                                                                  [ rdf:type owl:Restriction ;
                                                                    owl:onProperty :Instance_Description_has_Type ;
                                                                    owl:allValuesFrom :Complex_Data_Type
                                                                  ]
                                                                ) ;
                                             rdf:type owl:Class
                                           ] .


###  http://www.w3id.org/hsu-aut/DINEN61360#is_Type_Description_of_Data_Element
:is_Type_Description_of_Data_Element rdf:type owl:ObjectProperty ;
                                     rdfs:comment """Description:
ObjectProperty is used to connect a Type_Description with a Data_Element that has instace descriptions of this type. 

Inverse of has_Type_Description""" .


#################################################################
#    Data properties
#################################################################

###  http://www.w3id.org/hsu-aut/DINEN61360#Array_Member_Dimension
:Array_Member_Dimension rdf:type owl:DatatypeProperty ;
                        rdfs:domain :Array_Member ;
                        rdfs:range xsd:int ;
                        rdfs:comment """Description:

Indicates the dimension of an array member.""" .


###  http://www.w3id.org/hsu-aut/DINEN61360#Array_Member_Position
:Array_Member_Position rdf:type owl:DatatypeProperty ;
                       rdfs:comment """Description:

DataProperty that indicates the position of an Array_Member in a DataType List.""" .


###  http://www.w3id.org/hsu-aut/DINEN61360#Boolean_Operator
:Boolean_Operator rdf:type owl:DatatypeProperty ,
                           owl:FunctionalProperty ;
                  rdfs:range [ rdf:type rdfs:Datatype ;
                               owl:oneOf [ rdf:type rdf:List ;
                                           rdf:first "AND" ;
                                           rdf:rest [ rdf:type rdf:List ;
                                                      rdf:first "NAND" ;
                                                      rdf:rest [ rdf:type rdf:List ;
                                                                 rdf:first "NOR" ;
                                                                 rdf:rest [ rdf:type rdf:List ;
                                                                            rdf:first "OR" ;
                                                                            rdf:rest [ rdf:type rdf:List ;
                                                                                       rdf:first "XOR" ;
                                                                                       rdf:rest rdf:nil
                                                                                     ]
                                                                          ]
                                                               ]
                                                    ]
                                         ]
                             ] ;
                  rdfs:comment "Is used with Boolean_Association to define what kind of boolean relation connects the Data_Elements of the Boolean_Association" .


###  http://www.w3id.org/hsu-aut/DINEN61360#Code
:Code rdf:type owl:DatatypeProperty ;
      rdfs:subPropertyOf owl:topDataProperty ;
      rdf:type owl:FunctionalProperty ;
      rdfs:domain :Type_Description ;
      rdfs:comment """Description:
DIN EN 61360-1:2018 Section 7.3
Unique identifier of this data element type. Preferable this should be a standardized identifier (e.g. from eclss or common data dictionary).  optional exlusion of \"o\" and \"i\" is not implemented.    

Liability: necessary    

type: string with 6 digits between, first three digits are a-z and last three digits are 0-9  poposed data range expression: xsd:string[pattern \"[a-z0-9] {6}\"]""" .


###  http://www.w3id.org/hsu-aut/DINEN61360#Created_at_Date
:Created_at_Date rdf:type owl:DatatypeProperty ;
                 rdfs:domain :Instance_Description ;
                 rdfs:range xsd:dateTimeStamp ;
                 rdfs:comment """Description: 
A SemAnz40 attribute, that indicates the creation date for an instance.""" .


###  http://www.w3id.org/hsu-aut/DINEN61360#Definition
:Definition rdf:type owl:DatatypeProperty ;
            rdfs:subPropertyOf owl:topDataProperty ;
            rdfs:domain :Type_Description ;
            rdfs:comment """Description:
A textual definition of the data element

Liability: Necessary

DIN EN 61360-1:2018 Section 8.3

Type: String

Poposed Data Range Expression: xsd:string""" .


###  http://www.w3id.org/hsu-aut/DINEN61360#Drawing_Reference
:Drawing_Reference rdf:type owl:DatatypeProperty ;
                   rdfs:subPropertyOf owl:topDataProperty ;
                   rdfs:domain :Type_Description ;
                   rdfs:comment """Description:
A link to a drawing (or picture) that is used for further explanation of the data element

Liability: Optional

DIN EN 61360-1:2018 Section 6.13

Type: Contains a URL link as a string to a picture

Poposed Data Range Expression: xsd:string""" .


###  http://www.w3id.org/hsu-aut/DINEN61360#Expression_Goal
:Expression_Goal rdf:type owl:DatatypeProperty ;
                 rdfs:subPropertyOf owl:topDataProperty ;
                 rdf:type owl:FunctionalProperty ;
                 rdfs:domain :Instance_Description ;
                 rdfs:range [ rdf:type rdfs:Datatype ;
                              owl:oneOf [ rdf:type rdf:List ;
                                          rdf:first "Actual_Value" ;
                                          rdf:rest [ rdf:type rdf:List ;
                                                     rdf:first "Assurance" ;
                                                     rdf:rest [ rdf:type rdf:List ;
                                                                rdf:first "Requirement" ;
                                                                rdf:rest [ rdf:type rdf:List ;
                                                                           rdf:first "Variable" ;
                                                                           rdf:rest rdf:nil
                                                                         ]
                                                              ]
                                                   ]
                                        ]
                            ] ;
                 rdfs:comment """Description:

The goal of the values expression, which can be a Requirement against a value, an Assurance against a value, an actual (e.g. measured) value, or an unbound variable (e.g. without a concrete value).

Liability: Necessary""" .


###  http://www.w3id.org/hsu-aut/DINEN61360#Format_DIN61360_SemAnz40
:Format_DIN61360_SemAnz40 rdf:type owl:DatatypeProperty ;
                          rdfs:subPropertyOf owl:topDataProperty ;
                          rdfs:domain :Data_Element ;
                          rdfs:comment """Description: 

Indicates, whether the described type or entity is described by the DIN61360&SemAnz40 Format.

Liability: Necessary

Type: If true, the Data Element is based on the Din61360 and SemAnz40 description

Poposed Data Range Expression: xsd:boolean""" .


###  http://www.w3id.org/hsu-aut/DINEN61360#Formula
:Formula rdf:type owl:DatatypeProperty ;
         rdfs:subPropertyOf owl:topDataProperty ;
         rdfs:domain :Type_Description ;
         rdfs:comment """Description:
A mathematical euqation that is being used for characterization of the data element

Liability: Optional

DIN EN 61360-1:2018 Section 6.5

Type: contains a URL link as a string to a source file that describes the formula

Poposed Data Range Expression: xsd:string""" .


###  http://www.w3id.org/hsu-aut/DINEN61360#List_Member_Position
:List_Member_Position rdf:type owl:DatatypeProperty ;
                      rdfs:domain :List_Member ;
                      rdfs:range xsd:int ;
                      rdfs:comment """Description:

DataProperty that indicates the position of a List_Member in a DataType List.""" .


###  http://www.w3id.org/hsu-aut/DINEN61360#Logic_Interpretation
:Logic_Interpretation rdf:type owl:DatatypeProperty ;
                      rdfs:subPropertyOf owl:topDataProperty ;
                      rdf:type owl:FunctionalProperty ;
                      rdfs:domain :Instance_Description ;
                      rdfs:range [ rdf:type rdfs:Datatype ;
                                   owl:oneOf [ rdf:type rdf:List ;
                                               rdf:first "!=" ;
                                               rdf:rest [ rdf:type rdf:List ;
                                                          rdf:first "<" ;
                                                          rdf:rest [ rdf:type rdf:List ;
                                                                     rdf:first "<=" ;
                                                                     rdf:rest [ rdf:type rdf:List ;
                                                                                rdf:first "=" ;
                                                                                rdf:rest [ rdf:type rdf:List ;
                                                                                           rdf:first ">" ;
                                                                                           rdf:rest [ rdf:type rdf:List ;
                                                                                                      rdf:first ">=" ;
                                                                                                      rdf:rest rdf:nil
                                                                                                    ]
                                                                                         ]
                                                                              ]
                                                                   ]
                                                        ]
                                             ]
                                 ] ;
                      rdfs:comment """Description:

Indicates, whether a value with a certain Expression Goal has to be considered as equal (\"=\"), not equal (\"!=\"), greater than (\"<\"), lower than (\">\") or in combination with an equals (i.e. \"<=\", \">=\").

Liability: Necessary""" .


###  http://www.w3id.org/hsu-aut/DINEN61360#Note
:Note rdf:type owl:DatatypeProperty ;
      rdfs:subPropertyOf owl:topDataProperty ;
      rdfs:domain :Type_Description ;
      rdfs:comment """Description:
Additional information that are important to understand the meaning of the data element

Liability: Optional

DIN EN 61360-1:2018 Section 8.4

Type: String

Poposed Data Range Expression: xsd:string""" .


###  http://www.w3id.org/hsu-aut/DINEN61360#Preferred_Letter_Symbol
:Preferred_Letter_Symbol rdf:type owl:DatatypeProperty ;
                         rdfs:subPropertyOf owl:topDataProperty ;
                         rdfs:domain :Type_Description ;
                         rdfs:comment """Description:
A sign or literal that is used to represent the property (e.g. greek \"sigma\" for tension))

Liability: Optional

DIN EN 61360-1:2018 Section 6.6

Type: IEC 60027, IEC 60747 or IEC 60148 compliant formula sign described as a string

Poposed Data Range Expression: xsd:string""" .


###  http://www.w3id.org/hsu-aut/DINEN61360#Preferred_Name
:Preferred_Name rdf:type owl:DatatypeProperty ;
                rdfs:subPropertyOf owl:topDataProperty ;
                rdfs:domain :Type_Description ;
                rdfs:comment """Description:
Represents the preferred name of the data element type, that is being used for searches for instance.

Liability: Necessary

DIN EN 61360-1:2018 Section 7.4

Type: String with lower and upper case, with a maximum of 70 characters

Poposed Data Range Expression: xsd:string[maxLength 70]""" .


###  http://www.w3id.org/hsu-aut/DINEN61360#Quality
:Quality rdf:type owl:DatatypeProperty ;
         rdfs:subPropertyOf owl:topDataProperty ;
         rdfs:domain :Instance_Description ;
         rdfs:comment """Description:

Not supported so far, since it requires a additional quality ontology""" .


###  http://www.w3id.org/hsu-aut/DINEN61360#Remark
:Remark rdf:type owl:DatatypeProperty ;
        rdfs:domain :Type_Description ;
        rdfs:comment """Additional information that can be used to express a oppinion but should not change the meaning of the definition.
DIN EN 61360-1:2018 Section 8.5""" .


###  http://www.w3id.org/hsu-aut/DINEN61360#Revision_Number
:Revision_Number rdf:type owl:DatatypeProperty ;
                 rdfs:subPropertyOf owl:topDataProperty ;
                 rdfs:domain :Type_Description ;
                 rdfs:comment """Description:
Number that represents the actual count of changes

Liability: Necessary

DIN EN 61360-1:2018 Section 7.5

Type: Integer with two digits between 1 and 99

Poposed Data Range Expression: xsd:integer[>= 1 , <= 99]""" .


###  http://www.w3id.org/hsu-aut/DINEN61360#Short_Name
:Short_Name rdf:type owl:DatatypeProperty ;
            rdfs:subPropertyOf owl:topDataProperty ;
            rdfs:domain :Type_Description ;
            rdfs:comment """Description:
A short name or acronym that is used for the preferred name

Liability: Necessary

DIN EN 61360-1:2018 Section 7.6

Type: Strong restrictions of DIN61360  not implemented, just strings necessary. Maximum characters is 17.

Poposed Data Range Expression: xsd:string[maxLength 17]""" .


###  http://www.w3id.org/hsu-aut/DINEN61360#Source_Document_of_Definition
:Source_Document_of_Definition rdf:type owl:DatatypeProperty ;
                               rdfs:subPropertyOf owl:topDataProperty ;
                               rdfs:domain :Type_Description ;
                               rdfs:comment """Description:
A link to a source file, where the definition of the data element was taken from

Liability: Optional

DIN EN 61360-1:2018 Section 8.6

Type: Should contain a description of the source document with a maximum of 80 characters. Document has to be approved by ISO or IEC (e.g. should be a standard like IEC XXXXX). Alternatively use a URL to give a source document that is not approved by ISO.

Poposed Data Range Expression: xsd:string""" .


###  http://www.w3id.org/hsu-aut/DINEN61360#Synonymous_Letter_Symbol
:Synonymous_Letter_Symbol rdf:type owl:DatatypeProperty ;
                          rdfs:subPropertyOf owl:topDataProperty ;
                          rdfs:domain :Type_Description ;
                          rdfs:comment """Description:
A synonym that is used for the preferred equation sign

Liability: Optional

DIN EN 61360-1:2018 Section 6.7

Type: IEC 60027, IEC 60747 or IEC 60148 compliant formula sign

Poposed Data Range Expression: xsd:string""" .


###  http://www.w3id.org/hsu-aut/DINEN61360#Synonymous_Name
:Synonymous_Name rdf:type owl:DatatypeProperty ;
                 rdfs:subPropertyOf owl:topDataProperty ;
                 rdfs:domain :Type_Description ;
                 rdfs:comment """Description:
Synonyms to the preferred name

Liability: Optional

DIN EN 61360-1:2018 Section 7.7

Type: String with lower and upper case, with a maximum of 70 characters

Poposed Data Range Expression: xsd:string[maxLength 70]""" .


###  http://www.w3id.org/hsu-aut/DINEN61360#Unit_of_Measure
:Unit_of_Measure rdf:type owl:DatatypeProperty ;
                 rdfs:subPropertyOf owl:topDataProperty ;
                 rdfs:domain :Type_Description ;
                 rdfs:comment """Description:
Defines the unit of measure for a data element (e.g. km/h)

DIN EN 61360-1:2018 Section 10.7

Type: This data property represents the unit of measure, which should be ISO 31 compliant (SI-Units)

Poposed Data Range Expression: xsd:string""" .


###  http://www.w3id.org/hsu-aut/DINEN61360#Value
:Value rdf:type owl:DatatypeProperty ;
       rdfs:subPropertyOf owl:topDataProperty ;
       rdf:type owl:FunctionalProperty ;
       rdfs:domain [ owl:intersectionOf ( :Instance_Description
                                          [ rdf:type owl:Restriction ;
                                            owl:onProperty :Instance_Description_has_Type ;
                                            owl:allValuesFrom :Simple_Data_Type
                                          ]
                                        ) ;
                     rdf:type owl:Class
                   ] ;
       rdfs:comment """Description:

The actual value of something being described.

Liability: Necessary

SemAnz40

Type: This data property represents the value of the data element, which is a string, while the actual data type is represented by the Data Property DataType (!)

Poposed Data Range Expression: xsd:string""" .


###  http://www.w3id.org/hsu-aut/DINEN61360#Value_Format_Field_length
:Value_Format_Field_length rdf:type owl:DatatypeProperty ;
                           rdfs:subPropertyOf owl:topDataProperty ;
                           rdfs:domain :Type_Description ;
                           rdfs:comment """Description:
Defines the representation of a data element in length and kind. See DIN61360 for detailed description of possible formats. Possible definitions include non-quantitative formats, quantitative formats and maximum count of characters

Liability: Necessary

DIN EN 61360-1:2018 Section 10.8

Type: This data property represents only the field length, since this could be exponential (expressed with an E), it is a string

Poposed Data Range Expression: xsd:string""" .


###  http://www.w3id.org/hsu-aut/DINEN61360#Value_Format_Field_length_Variable
:Value_Format_Field_length_Variable rdf:type owl:DatatypeProperty ;
                                    rdfs:subPropertyOf owl:topDataProperty ;
                                    rdfs:domain :Type_Description ;
                                    rdfs:comment """Description:
Defines the representation of a data element in length and kind. See DIN61360 for detailed description of possible formats. Possible definitions include non-quantitative formats, quantitative formats and maximum count of characters

Liability: Necessary

DIN EN 61360-1:2018 Section 10.8

Type: This data property represents only the case, that a value format has a variable field length (true)

Poposed Data Range Expression: xsd:boolean""" .


###  http://www.w3id.org/hsu-aut/DINEN61360#Value_Format_non-quantitativ
:Value_Format_non-quantitativ rdf:type owl:DatatypeProperty ;
                              rdfs:subPropertyOf owl:topDataProperty ;
                              rdfs:domain :Type_Description ;
                              rdfs:range [ rdf:type rdfs:Datatype ;
                                           owl:oneOf [ rdf:type rdf:List ;
                                                       rdf:first "A" ;
                                                       rdf:rest [ rdf:type rdf:List ;
                                                                  rdf:first "B" ;
                                                                  rdf:rest [ rdf:type rdf:List ;
                                                                             rdf:first "M" ;
                                                                             rdf:rest [ rdf:type rdf:List ;
                                                                                        rdf:first "N" ;
                                                                                        rdf:rest [ rdf:type rdf:List ;
                                                                                                   rdf:first "X" ;
                                                                                                   rdf:rest rdf:nil
                                                                                                 ]
                                                                                      ]
                                                                           ]
                                                                ]
                                                     ]
                                         ] ;
                              owl:propertyDisjointWith :Value_Format_quantitativ ;
                              rdfs:comment """Description:
Defines the representation of a data element in length and kind. See DIN61360 for detailed description of possible formats. Possible definitions include non-quantitative formats, quantitative formats and maximum count of characters

Liability: Necessary

DIN EN 61360-1:2018 Section 10.8

Type: This data property represents only the non-quantitativ formats, string

Poposed Data Range Expression: xsd:string""" .


###  http://www.w3id.org/hsu-aut/DINEN61360#Value_Format_quantitativ
:Value_Format_quantitativ rdf:type owl:DatatypeProperty ;
                          rdfs:subPropertyOf owl:topDataProperty ;
                          rdfs:domain :Type_Description ;
                          rdfs:range [ rdf:type rdfs:Datatype ;
                                       owl:oneOf [ rdf:type rdf:List ;
                                                   rdf:first "NR1" ;
                                                   rdf:rest [ rdf:type rdf:List ;
                                                              rdf:first "NR2" ;
                                                              rdf:rest [ rdf:type rdf:List ;
                                                                         rdf:first "NR3" ;
                                                                         rdf:rest rdf:nil
                                                                       ]
                                                            ]
                                                 ]
                                     ] ;
                          rdfs:comment """Description:
Defines the representation of a data element in length and kind. See DIN61360 for detailed description of possible formats. Possible definitions include non-quantitative formats, quantitative formats and maximum count of characters

Liability: Necessary

DIN EN 61360-1:2018 Section 10.8

Type: This data property represents only the quantitativ formats, string

Poposed Data Range Expression: xsd:string""" .


###  http://www.w3id.org/hsu-aut/DINEN61360#Value_List
:Value_List rdf:type owl:DatatypeProperty ;
            rdfs:subPropertyOf owl:topDataProperty ;
            rdfs:domain :Simple_Data_Type ;
            rdfs:comment """Description: 
Represents the possible values for a data element

Liability: optional (in DIN613060 case depended due to classification of data element, which is not implemented here)

DIN EN 61360-1:2018 Section 16

Type: This data property represents the information, if there is a value list (if so, true), basically the values that the data property \"Value\" is allowed to hold. 

Poposed Data Range Expression: xsd:boolean""" .


###  http://www.w3id.org/hsu-aut/DINEN61360#Value_List_Member
:Value_List_Member rdf:type owl:DatatypeProperty ;
                   rdfs:subPropertyOf owl:topDataProperty ;
                   rdfs:domain :Simple_Data_Type ;
                   rdfs:comment """Description: 
Represents the possible values for a data element

Liability: optional (in DIN613060 case depended due to classification of data element, which is not implemented here)

DIN EN 61360-1:2018 Section 16

Poposed Data Range Expression: xsd:string""" .


###  http://www.w3id.org/hsu-aut/DINEN61360#Version_Number
:Version_Number rdf:type owl:DatatypeProperty ;
                rdfs:subPropertyOf owl:topDataProperty ;
                rdfs:domain :Type_Description ;
                rdfs:comment """Description:
Number that indicates different versions of one data element type

Liability: Necessary

DIN EN 61360-1:2018 Section 7.8

Type: Integer with three digits max, so between 1 and 999

Poposed Data Range Expression: xsd:integer[>= 1 , <= 999]""" .


###  http://www.w3id.org/hsu-aut/DINEN61360#backwards_compatible_Revision
:backwards_compatible_Revision rdf:type owl:DatatypeProperty ;
                               rdfs:domain :Type_Description ;
                               rdfs:comment """Description:
Indicates, to which revisions the data type is backwards compatible.

Type: Integer

Poposed Data Range Expression: xsd:string""" .


###  http://www.w3id.org/hsu-aut/DINEN61360#backwards_compatible_Version
:backwards_compatible_Version rdf:type owl:DatatypeProperty ;
                              rdfs:domain :Type_Description ;
                              rdfs:comment """Description:
Indicates, to which version numbers the data type is backwards compatible.

Type: Integer

Poposed Data Range Expression: xsd:string""" .


#################################################################
#    Classes
#################################################################

###  http://www.w3id.org/hsu-aut/DINEN61360#Array
:Array rdf:type owl:Class ;
       rdfs:subClassOf :Complex_Data_Type ,
                       [ rdf:type owl:Restriction ;
                         owl:onProperty :complex_Data_Type_has_Member ;
                         owl:allValuesFrom :Array_Member
                       ] .


###  http://www.w3id.org/hsu-aut/DINEN61360#Array_Member
:Array_Member rdf:type owl:Class ;
              rdfs:subClassOf :Complex_Data_Type_Member ,
                              [ rdf:type owl:Restriction ;
                                owl:onProperty :Array_Member_Dimension ;
                                owl:qualifiedCardinality "1"^^xsd:nonNegativeInteger ;
                                owl:onDataRange xsd:int
                              ] ,
                              [ rdf:type owl:Restriction ;
                                owl:onProperty :Array_Member_Position ;
                                owl:qualifiedCardinality "1"^^xsd:nonNegativeInteger ;
                                owl:onDataRange xsd:int
                              ] .


###  http://www.w3id.org/hsu-aut/DINEN61360#Bag
:Bag rdf:type owl:Class ;
     rdfs:subClassOf :Complex_Data_Type ,
                     [ rdf:type owl:Restriction ;
                       owl:onProperty :complex_Data_Type_has_Member ;
                       owl:allValuesFrom :Bag_Member
                     ] .


###  http://www.w3id.org/hsu-aut/DINEN61360#Bag_Member
:Bag_Member rdf:type owl:Class ;
            rdfs:subClassOf :Complex_Data_Type_Member .


###  http://www.w3id.org/hsu-aut/DINEN61360#Boolean
:Boolean rdf:type owl:Class ;
         rdfs:subClassOf :Simple_Data_Type ,
                         [ rdf:type owl:Restriction ;
                           owl:onProperty :Value_List_Member ;
                           owl:allValuesFrom xsd:boolean
                         ] .


###  http://www.w3id.org/hsu-aut/DINEN61360#Complex_Data_Type
:Complex_Data_Type rdf:type owl:Class ;
                   rdfs:subClassOf :Data_Type ;
                   owl:disjointWith :Simple_Data_Type .


###  http://www.w3id.org/hsu-aut/DINEN61360#Complex_Data_Type_Member
:Complex_Data_Type_Member rdf:type owl:Class ;
                          rdfs:subClassOf :Data_Type .


###  http://www.w3id.org/hsu-aut/DINEN61360#Data_Element
:Data_Element rdf:type owl:Class ;
              rdfs:subClassOf [ rdf:type owl:Restriction ;
                                owl:onProperty :has_Type_Description ;
                                owl:someValuesFrom :Type_Description
                              ] ,
                              [ rdf:type owl:Restriction ;
                                owl:onProperty :has_Instance_Description ;
                                owl:minQualifiedCardinality "0"^^xsd:nonNegativeInteger ;
                                owl:onClass :Instance_Description
                              ] ;
              owl:disjointWith :Type_Description ;
              rdfs:comment """Description:
Contains a the structure of all data element (DIN61360 3.5.2, see also section 4)

Each Data_Element has to have a type description and may have an instance description""" .


###  http://www.w3id.org/hsu-aut/DINEN61360#Data_Type
:Data_Type rdf:type owl:Class .


###  http://www.w3id.org/hsu-aut/DINEN61360#Instance_Description
:Instance_Description rdf:type owl:Class ;
                      rdfs:subClassOf [ rdf:type owl:Restriction ;
                                        owl:onProperty :Expression_Goal ;
                                        owl:qualifiedCardinality "1"^^xsd:nonNegativeInteger ;
                                        owl:onDataRange xsd:string
                                      ] ,
                                      [ rdf:type owl:Restriction ;
                                        owl:onProperty :Logic_Interpretation ;
                                        owl:qualifiedCardinality "1"^^xsd:nonNegativeInteger ;
                                        owl:onDataRange xsd:string
                                      ] ;
                      owl:disjointWith :Type_Description .


###  http://www.w3id.org/hsu-aut/DINEN61360#Integer
:Integer rdf:type owl:Class ;
         rdfs:subClassOf :Simple_Data_Type ,
                         [ rdf:type owl:Restriction ;
                           owl:onProperty :Value_List_Member ;
                           owl:allValuesFrom xsd:int
                         ] .


###  http://www.w3id.org/hsu-aut/DINEN61360#List
:List rdf:type owl:Class ;
      rdfs:subClassOf :Complex_Data_Type ,
                      [ rdf:type owl:Restriction ;
                        owl:onProperty :complex_Data_Type_has_Member ;
                        owl:allValuesFrom :List_Member
                      ] .


###  http://www.w3id.org/hsu-aut/DINEN61360#List_Member
:List_Member rdf:type owl:Class ;
             rdfs:subClassOf :Complex_Data_Type_Member ,
                             [ rdf:type owl:Restriction ;
                               owl:onProperty :List_Member_Position ;
                               owl:qualifiedCardinality "1"^^xsd:nonNegativeInteger ;
                               owl:onDataRange xsd:int
                             ] .


###  http://www.w3id.org/hsu-aut/DINEN61360#Real
:Real rdf:type owl:Class ;
      rdfs:subClassOf :Simple_Data_Type ,
                      [ rdf:type owl:Restriction ;
                        owl:onProperty :Value_List_Member ;
                        owl:allValuesFrom xsd:float
                      ] .


###  http://www.w3id.org/hsu-aut/DINEN61360#Set
:Set rdf:type owl:Class ;
     rdfs:subClassOf :Complex_Data_Type ,
                     [ rdf:type owl:Restriction ;
                       owl:onProperty :complex_Data_Type_has_Member ;
                       owl:allValuesFrom :Set_Member
                     ] .


###  http://www.w3id.org/hsu-aut/DINEN61360#Set_Member
:Set_Member rdf:type owl:Class ;
            rdfs:subClassOf :Complex_Data_Type_Member .


###  http://www.w3id.org/hsu-aut/DINEN61360#Simple_Data_Type
:Simple_Data_Type rdf:type owl:Class ;
                  rdfs:subClassOf :Data_Type ,
                                  [ rdf:type owl:Restriction ;
                                    owl:onProperty :Value_List ;
                                    owl:qualifiedCardinality "1"^^xsd:nonNegativeInteger ;
                                    owl:onDataRange xsd:boolean
                                  ] ;
                  rdfs:comment """Description:
Indicates which kind of DataType a data element must be. This does not include all data types of DIN61360! 

Liability: Necessary

DIN61360: 3.4.1

Type: is a enumeration of standard compliant data types. Please see DIN61360 for a description of level/class-instance/list/set/bag/array""" .


###  http://www.w3id.org/hsu-aut/DINEN61360#String
:String rdf:type owl:Class ;
        rdfs:subClassOf :Simple_Data_Type ,
                        [ rdf:type owl:Restriction ;
                          owl:onProperty :Value_List_Member ;
                          owl:allValuesFrom xsd:string
                        ] .


###  http://www.w3id.org/hsu-aut/DINEN61360#Type_Description
:Type_Description rdf:type owl:Class ;
                  rdfs:subClassOf [ rdf:type owl:Restriction ;
                                    owl:onProperty :Code ;
                                    owl:qualifiedCardinality "1"^^xsd:nonNegativeInteger ;
                                    owl:onDataRange xsd:string
                                  ] ,
                                  [ rdf:type owl:Restriction ;
                                    owl:onProperty :Definition ;
                                    owl:qualifiedCardinality "1"^^xsd:nonNegativeInteger ;
                                    owl:onDataRange xsd:string
                                  ] ,
                                  [ rdf:type owl:Restriction ;
                                    owl:onProperty :Preferred_Name ;
                                    owl:qualifiedCardinality "1"^^xsd:nonNegativeInteger ;
                                    owl:onDataRange xsd:string
                                  ] ,
                                  [ rdf:type owl:Restriction ;
                                    owl:onProperty :Short_Name ;
                                    owl:qualifiedCardinality "1"^^xsd:nonNegativeInteger ;
                                    owl:onDataRange xsd:string
                                  ] ,
                                  [ rdf:type owl:Restriction ;
                                    owl:onProperty :Version_Number ;
                                    owl:qualifiedCardinality "1"^^xsd:nonNegativeInteger ;
                                    owl:onDataRange xsd:int
                                  ] ,
                                  [ rdf:type owl:Restriction ;
                                    owl:onProperty :Preferred_Letter_Symbol ;
                                    owl:maxQualifiedCardinality "1"^^xsd:nonNegativeInteger ;
                                    owl:onDataRange xsd:string
                                  ] ,
                                  [ rdf:type owl:Restriction ;
                                    owl:onProperty :Synonymous_Letter_Symbol ;
                                    owl:maxQualifiedCardinality "2"^^xsd:nonNegativeInteger ;
                                    owl:onDataRange xsd:string
                                  ] ,
                                  [ rdf:type owl:Restriction ;
                                    owl:onProperty :Synonymous_Name ;
                                    owl:maxQualifiedCardinality "2"^^xsd:nonNegativeInteger ;
                                    owl:onDataRange xsd:string
                                  ] ;
                  rdfs:comment "Value list is expressed as exactly 1, since not using a value list has to result in value list false" .


#################################################################
#    Annotations
#################################################################

owl:Thing rdfs:comment """In order to check consistency, the following procedure is used:

First, the reasoner checks, whether the class expressions to hold for the ABox. If that is not the case, then a explanation of inconsistency can be accessed.

Second, SWRL rules are used to check the constency aspects that cannot be modelled through class expressions. These rules infer 4 \"Overall_X_Constent\" DataProperties. For the case that incremental rules were possible, other consistency attributes are inferred, so that in case of inconsistency a debugging can be started.

Explanation to class expressions in relation to DIN61360 definitions:

\"exactly\" is used for \"necessary\" (zwingend)
\"max\" is used for \"optinal\" (wahlfrei) with maximum restriction

If something is just \"optional\", it will not occur in the class expression.

If a liability in DIN61360 states \"case dependend\" (bedingt), then this considered in a SWRL rule, which will give the DataProperties of \"x_Consistent\" to the Data_Element""" .


#################################################################
#    General axioms
#################################################################

[ rdf:type owl:AllDisjointClasses ;
  owl:members ( :Array
                :Bag
                :Boolean
                :Integer
                :List
                :Real
                :Set
                :String
              )
] .


###  Generated by the OWL API (version 4.5.26.2023-07-17T20:34:13Z) https://github.com/owlcs/owlapi
